src/Language/PlutusIR/Semantics/Static/Normalisation.v
@@ -1,0 +1,247 @@
+Require Import PlutusCert.Language.PlutusIR.
+Import NamedTerm.
+
+Import Coq.Lists.List.
+Import Coq.Strings.String.
+
+Require Export PlutusCert.Language.PlutusIR.Semantics.Static.Implementations.
+
+
+
+(** ** Type equality *)
+Reserved Notation "T1 '=b' T2" (at level 40).
+Inductive EqT : Ty -> Ty -> Prop :=
+  (* Beta-reduction *)
+  | Q_Beta : forall X K T1 T2 T1',
+      substituteTCA X T2 T1 = T1' ->
+      Ty_App (Ty_Lam X K T1) T2 =b T1'
+  (* Reflexivity, Symmetry and Transitivity*)
+  | Q_Refl : forall T,
+      T =b T
+  | Q_Symm : forall T S,
+      T =b S ->
+      S =b T
+  | Q_Trans : forall S U T,
+      S =b U ->
+      U =b T ->
+      S =b T
+  (* Congruence *)
+  | Q_Fun : forall S1 S2 T1 T2,
+      S1 =b S2 ->
+      T1 =b T2 ->
+      Ty_Fun S1 T1 =b Ty_Fun S2 T2
+  | Q_Forall : forall X K S T,
+      S =b T ->
+      Ty_Forall X K S =b Ty_Forall X K T
+  | Q_Lam : forall X K S T,
+      S =b T ->
+      Ty_Lam X K S =b Ty_Lam X K T
+  | Q_App : forall S1 S2 T1 T2,
+      S1 =b S2 ->
+      T1 =b T2 ->
+      Ty_App S1 T1 =b Ty_App S2 T2
+where "T1 '=b' T2" := (EqT T1 T2).
+
+
+(** ** Normal types *)
+
+Inductive normal_Ty : Ty -> Prop :=
+  | NO_TyLam : forall bX K T,
+      normal_Ty T ->
+      normal_Ty (Ty_Lam bX K T)
+  | NO_neutral : forall T,
+      neutral_Ty T ->
+      normal_Ty T
+  | NO_TyFun : forall T1 T2,
+      normal_Ty T1 ->
+      normal_Ty T2 ->
+      normal_Ty (Ty_Fun T1 T2)
+  | NO_TyForall : forall bX K T,
+      normal_Ty T ->
+      normal_Ty (Ty_Forall bX K T)
+  | NO_TyIFix : forall F T,
+      normal_Ty F ->
+      normal_Ty T ->
+      normal_Ty (Ty_IFix F T)
+  | NO_TyBuiltin : forall st,
+      normal_Ty (Ty_Builtin st)
+
+with neutral_Ty : Ty -> Prop :=
+  | NE_TyVar : forall X,
+      neutral_Ty (Ty_Var X)
+  | NE_TyApp : forall T1 T2,
+      neutral_Ty T1 ->
+      normal_Ty T2 ->
+      neutral_Ty (Ty_App T1 T2).
+
+Scheme normal_Ty__ind := Minimality for normal_Ty Sort Prop
+  with neutral_Ty__ind := Minimality for neutral_Ty Sort Prop.
+
+Combined Scheme normal_Ty__multind from 
+  normal_Ty__ind,
+  neutral_Ty__ind.
+
+#[export] Hint Constructors normal_Ty neutral_Ty : core.
+
+Inductive is_TyLam : Ty -> Prop :=
+  | Is_TyLam : forall bX K T_body,
+      is_TyLam (Ty_Lam bX K T_body).
+
+#[export] Hint Constructors is_TyLam : core.
+
+(*
+Equations? normalise (T : Ty) : Ty :=
+  normalise (Ty_App T1 T2) =>
+    match normalise T1 with
+    | Ty_Lam bX K T1_body =>
+        normalise (substituteTCA bX (normalise T2) T1_body)
+    | T1' =>
+        Ty_App T1' (normalise T2)
+    end ;
+  normalise (Ty_Fun T1 T2) =>
+    Ty_Fun (normalise T1) (normalise T2) ;
+  normalise (Ty_Forall bX K T0) =>
+    Ty_Forall bX K (normalise T0) ;
+  normalise (Ty_Lam bX K T0) =>
+    Ty_Lam bX K (normalise T0) ;
+  normalise (Ty_Var X) =>
+    Ty_Var X ;
+  normalise (Ty_IFix F T) =>
+    Ty_IFix (normalise F) (normalise T) ;
+  normalise (Ty_Builtin st) =>
+    Ty_Builtin st
+  .
+*)
+
+Inductive normalise : Ty -> Ty -> Prop :=
+  | N_BetaReduce : forall bX K T1 T2 T1_body T2' T' T'',
+      normalise T1 (Ty_Lam bX K T1_body) ->
+      normalise T2 T2' ->
+      substituteTCA bX T2' T1_body = T' ->
+      normalise T' T'' ->
+      normalise (Ty_App T1 T2) T''
+  | N_TyApp : forall T1 T2 T1' T2',
+      neutral_Ty T1' ->
+      normalise T1 T1' ->
+      normalise T2 T2' ->
+      normalise (Ty_App T1 T2) (Ty_App T1' T2')
+  | N_TyFun : forall T1 T2 T1' T2',
+      normalise T1 T1' ->
+      normalise T2 T2' ->
+      normalise (Ty_Fun T1 T2) (Ty_Fun T1' T2')
+  | N_TyForall : forall bX K T0 T0',
+      normalise T0 T0' ->
+      normalise (Ty_Forall bX K T0) (Ty_Forall bX K T0')
+  | N_TyLam : forall bX K T0 T0',
+      normalise T0 T0' ->
+      normalise (Ty_Lam bX K T0) (Ty_Lam bX K T0')
+  | N_TyVar : forall X,
+      normalise (Ty_Var X) (Ty_Var X)
+  | N_TyIFix : forall F T F' T',
+      normalise F F' ->
+      normalise T T' ->
+      normalise (Ty_IFix F T) (Ty_IFix F' T')
+  | N_TyBuiltin : forall st,
+      normalise (Ty_Builtin st) (Ty_Builtin st)
+  .
+
+#[export] Hint Constructors normalise : core.
+
+Lemma normalise_deterministic : forall T T_norm T'_norm,
+  normalise T T_norm ->
+  normalise T T'_norm ->
+  T_norm = T'_norm.
+Proof.
+  intros.
+  generalize dependent T'_norm.
+  induction H; intros.
+  - inversion H3.
+    + subst.
+      apply IHnormalise1 in H6. inversion H6. subst.
+      apply IHnormalise2 in H7. subst.
+      apply IHnormalise3; eauto.
+    + subst.
+      apply IHnormalise1 in H7. 
+      inversion H7. subst.
+      inversion H6.
+  - inversion H2.
+    + subst.
+      apply IHnormalise1 in H5.
+      inversion H5. subst.
+      inversion H.
+    + subst.
+      f_equal; eauto.
+  - inversion H1. subst.
+    f_equal; eauto.
+  - inversion H0. subst.
+    f_equal; eauto.
+  - inversion H0. subst.
+    f_equal; eauto.
+  - inversion H0. subst.
+    f_equal; eauto.
+  - inversion H1. subst.
+    f_equal; eauto.
+  - inversion H0. subst.
+    eauto.
+Qed.
+
+Lemma normalise_to_normal : forall T T_norm,
+    normalise T T_norm ->
+    normal_Ty T_norm.
+Proof. 
+  induction 1; eauto.
+Qed.
+
+Lemma normalisation__completeness : forall S T S_norm T_norm,
+  S =b T ->
+  normalise S S_norm ->
+  normalise T T_norm ->
+  S_norm = T_norm.
+Proof. Admitted.
+
+Theorem normalisation__soundness : forall T T_norm,
+    normalise T T_norm ->
+    T =b T_norm.
+Proof. Admitted.
+
+Theorem normalisation__stability : forall T T_norm,
+    normal_Ty T ->
+    normalise T T_norm ->
+    T = T_norm.
+Proof. Admitted.
+
+
+Inductive map_normalise : list (tyname * Ty) -> list (tyname * Ty) -> Prop :=
+  | MN_nil : 
+      map_normalise nil nil
+  | MN_cons : forall X T Ts Tn Tsn,
+      map_normalise Ts Tsn ->
+      normalise T Tn ->
+      map_normalise ((X, T) :: Ts) ((X, Tn) :: Tsn).
+
+#[export] Hint Constructors map_normalise : core.
+
+Lemma map_normalise__app : forall l1 l2 ln,
+    map_normalise (l1 ++ l2) ln ->
+    exists l1n l2n, 
+      map_normalise l1 l1n /\
+      map_normalise l2 l2n /\
+      ln = l1n ++ l2n.
+Proof.
+  induction l1; intros.
+  - exists nil. exists ln. eauto.
+  - inversion H. subst.
+    eapply IHl1 in H2.
+    destruct H2 as [l1n' [l2n' [Hmn1 [Hmn2 Heq]]]].
+    subst.
+    exists ((X, Tn) :: l1n').
+    exists l2n'.
+    eauto.
+Qed.
+
+
+Lemma map_normalise__deterministic : forall l ln ln',
+    map_normalise l ln ->
+    map_normalise l ln' ->
+    ln = ln'.
+Proof. Admitted.
