src/Language/PlutusIR/Transform/LetNonRec/SSP.v
@@ -26,10 +26,11 @@ Definition P_bindings_well_formed_nonrec Delta Gamma bs1 :=
       map binds_Delta bs1 = map binds_Delta bs2 /\
       map binds_Gamma bs1 = map binds_Gamma bs2
     ) /\ (
-      forall f_bs2 t T,
+      forall f_bs2 t T bs1Gn,
         Delta ,, Gamma |-oks_nr bs1 -> 
         CNR_Bindings bs1 f_bs2 ->
-        (mupdate Delta (flatten (map binds_Delta bs1))) ,, (mupdate Gamma (flatten (map binds_Gamma bs1))) |-+ t : T ->
+        map_normalise (flatten (map binds_Gamma bs1)) bs1Gn ->
+        (mupdate Delta (flatten (map binds_Delta bs1))) ,, (mupdate Gamma bs1Gn) |-+ t : T ->
         Delta ,, Gamma |-+ (fold_right apply t f_bs2) : T
     ).
 
@@ -54,10 +55,11 @@ Definition P_binding_well_formed Delta Gamma b1 :=
       binds_Delta b1 = binds_Delta b2 /\
       binds_Gamma b1 = binds_Gamma b2
     ) /\ (
-      forall f_b2 t T,
+      forall f_b2 t T bs1Gn,
         Delta ,, Gamma |-ok b1 ->
         CNR_Binding b1 f_b2 ->
-        mupdate Delta (binds_Delta b1) ,, mupdate Gamma (binds_Gamma b1) |-+ t : T ->
+        map_normalise (binds_Gamma b1) bs1Gn ->
+        mupdate Delta (binds_Delta b1) ,, mupdate Gamma bs1Gn |-+ t : T ->
         Delta ,, Gamma |-+ (f_b2 t) : T  
     ).
 
@@ -82,44 +84,57 @@ Proof.
   all: intros; autounfold; intros.
   - (* T_Let *)
     inversion X; subst.
-    + apply H2.
+    + eapply H3.
       * apply bs.
       * assumption.
       * assumption.
-      * apply H4.
+      * eassumption.
+      * apply H5.
         assumption.
     + inversion X0. subst. 
       eapply T_Let.
       * reflexivity.
+      * unfold P_bindings_well_formed_nonrec in H3.
+        edestruct H3 as [_ [Heq _]].
+        apply Heq in X1.
+        destruct X1.
+        rewrite <- H1.
+        eassumption.
       * reflexivity.
-      * apply H2. assumption. assumption.
-      * unfold P_bindings_well_formed_rec in H2. edestruct H2 as [_ [Heq _]]. apply Heq in X1. 
-        destruct X1. rewrite <- H. rewrite <- H0. apply H4. assumption. 
+      * apply H3. assumption. assumption.
+      * unfold P_bindings_well_formed_nonrec in H3. edestruct H3 as [_ [Heq _]]. apply Heq in X1. 
+        destruct X1. rewrite <- H. apply H5. assumption. 
   - (* T_LetRec *)
     inversion X. subst.
     inversion X0. subst.
     eapply T_LetRec.
     + reflexivity.
+    + unfold P_bindings_well_formed_rec in H3.
+      edestruct H3 as [IHH Heq].
+      apply Heq in X1 as Hsu.
+      destruct Hsu.
+      rewrite <- H1.
+      eassumption.
     + reflexivity.
-    + unfold P_bindings_well_formed_rec in H1.
-      edestruct H2 as [IHH Heq].
+    + unfold P_bindings_well_formed_rec in H3.
+      edestruct H3 as [IHH Heq].
       apply Heq in X1 as Hsu.
       destruct Hsu.
       rewrite <- H.
-      rewrite <- H0.
       apply IHH. auto. auto.
-    + unfold P_bindings_well_formed_rec in H1.
-      edestruct H2 as [IHH Heq].
+    + unfold P_bindings_well_formed_rec in H3.
+      edestruct H3 as [IHH Heq].
       apply Heq in X1 as Hsu.
       destruct Hsu.
       rewrite <- H.
-      rewrite <- H0.
-      apply H4.
+      apply H5.
       assumption.
   - (* T_Var *)
     inversion X. subst.
     inversion X0. subst.
-    apply T_Var. assumption.
+    apply T_Var with T. 
+    assumption.
+    assumption.
   - (* T_TyAbs *)
     inversion X0. subst.
     inversion X1. subst.
@@ -131,12 +146,13 @@ Proof.
     inversion X. subst.
     inversion X0. subst.
     apply T_LamAbs.
-    + apply H0. assumption.
     + assumption.
+    + assumption.
+    + apply H2. assumption.
   - (* T_Apply *)
     inversion X. subst.
     inversion X0. subst.
-    apply T_Apply with T1.
+    apply T_Apply with T1n.
     + apply H0. assumption.
     + apply H2. assumption.
   - (* T_Constant *)
@@ -151,7 +167,7 @@ Proof.
   - (* T_TyInst *)
     inversion X0. subst.
     inversion X1. subst.
-    apply T_TyInst with (T1 := T1) (X := X) (K2 := K2) (T1' := T1').
+    apply T_TyInst with T1n X K2 T2n.
     + apply H0. assumption.
     + assumption.
     + assumption.
@@ -160,23 +176,26 @@ Proof.
     inversion X. subst.
     inversion X0. subst.
     apply T_Error.
-    apply H.
+    assumption.
+    assumption.
   - (* T_IWrap *)
     inversion X. subst.
     inversion X0. subst.
-    apply T_IWrap with (K := K) (S := S).
+    apply T_IWrap with K T0n.
     + assumption.
     + apply H1. assumption.
+    + assumption.
+    + assumption.
     + assumption.
     + assumption.
   - (* T_Unwrap *)
     inversion X. subst.
     inversion X0. subst.
-    apply T_Unwrap with (F := F) (K := K) (T := T).
+    apply T_Unwrap with Fn K Tn.
     + apply H0. assumption.
     + assumption.
     + assumption.
-
+    
   - (* T_ExtBuiltin *)
     inversion X. subst.
     inversion X0.
@@ -196,20 +215,26 @@ Proof.
       * intros.
         inversion X. subst.
         simpl in H0.
+        inversion H0. subst.
         assumption.
   - (* W_ConsB_NonRec *)
     split.
     + intros.
       inversion X. subst.
-      apply W_ConsB_NonRec.
+      eapply W_ConsB_NonRec.
       * apply H0. assumption. assumption.
       * unfold P_binding_well_formed in H0.
         edestruct H0 as [_ [Heq _]].
         apply Heq in X0.
         destruct X0.
-        rewrite <- H4.
+        rewrite <- H6.
+        eassumption.
+      * unfold P_binding_well_formed in H0.
+        edestruct H0 as [_ [Heq _]].
+        apply Heq in X0.
+        destruct X0.
         rewrite <- H5.
-        apply H2. assumption. assumption.
+        apply H3. assumption. assumption.
     + split.
       * intros.
         inversion X. subst.
@@ -217,34 +242,46 @@ Proof.
         split.
         -- f_equal.
            ++ apply H0. assumption.
-           ++ apply H2. assumption.
+           ++ apply H3. assumption.
         -- f_equal.
            ++ apply H0. assumption.
-           ++ apply H2. assumption.
+           ++ apply H3. assumption.
       * intros.
         inversion X. subst.
         inversion X0. subst.
-        edestruct H2 as [_ [_ J]].
+        edestruct H3 as [_ [_ J]].
         
         simpl.
         edestruct H0 as [_ [_ J2]].
-        apply J2.
+        eapply J2.
         -- assumption.
         -- assumption.
-        -- apply J.
+        -- eassumption.
+        -- unfold flatten in H5.
+            simpl in H5.
+            rewrite concat_app in H5.
+            simpl in H5.
+            apply map_normalise__app in H5 as H20. 
+            destruct H20 as [l1n [l2n [Hmn1 [Hmn2 Heq]]]].
+            subst. 
+
+          eapply J.
            ++ assumption.
            ++ assumption.
+           ++ eauto.
            ++ simpl.
-              simpl in H4.
-              unfold flatten in H4.
-              simpl in H4.  
-              rewrite concat_app in H4.
-              simpl in H4.
-              rewrite app_nil_r in H4.
-              rewrite concat_app in H4.
-              rewrite mupdate_app in H4.
-              simpl in H4.
-              apply H4.
+              simpl in H6.
+              unfold flatten in H6.
+              simpl in H6.  
+              rewrite concat_app in H6.
+              simpl in H6.
+              rewrite app_nil_r in H6.
+              rewrite mupdate_app in H6.
+              simpl in H6.
+              simpl in H1.
+              eapply map_normalise__deterministic in H1; eauto.
+              subst.
+              apply H6.
   - (* W_NilB_Rec *)
     split.
     + intros.
@@ -284,12 +321,24 @@ Proof.
         auto.
       * intros.
         inversion X. subst.
+        apply strong_normalisation in H as He.
+        destruct He.
         eapply T_Apply.
         -- apply T_LamAbs.
           ++ simpl in H3.
              assumption. 
-          ++ assumption.
-        -- apply H1. assumption.
+          ++ apply H5.
+          ++ simpl in H4.
+             simpl in H3.
+             inversion H3. subst.
+             inversion H10. subst.
+             eapply normalise_deterministic in H5; eauto.
+             subst.
+             simpl in H4.
+            eassumption.
+        -- apply has_type__normal in H0 as H10.
+           eapply normalisation__stability in H10; eauto.
+           subst. eapply H1. assumption.
   - (* W_Type *)
     split.
     + intros. 
